Begin adding sequence conversions

Sequences/IntSeq.dfy
@@ -1,5 +1,3 @@
-/* Little endian representation */
-
 include "../Nonlinear_Arithmetic/DivMod.dfy"
 include "../Nonlinear_Arithmetic/Mul.dfy"
 include "../NativeTypes.dfy"
@@ -34,7 +32,7 @@ module IntSeq {
   }
 
   /* Proves the nat representation of a sequence of length 1. */
-  lemma lemma_to_nat_len_1(xs: seq<BaseType>)
+  lemma lemma_seq_len_1_nat(xs: seq<BaseType>)
     requires |xs| == 1
     ensures to_nat(xs) == xs[0]
   {
@@ -43,18 +41,25 @@ module IntSeq {
   }
 
   /* Proves the nat representation of a sequence of length 2. */
-  lemma lemma_to_nat_len_2(xs: seq<BaseType>)
+  lemma lemma_seq_len_2_nat(xs: seq<BaseType>)
     requires |xs| == 2
     ensures to_nat(xs) == xs[0] + xs[1] * BASE
   {
     reveal to_nat();
-    lemma_to_nat_len_1(drop_last(xs));
+    lemma_seq_len_1_nat(drop_last(xs));
     reveal power();
+  }
+
+  lemma lemma_seq_equivalence(xs: seq<BaseType>, ys: seq<BaseType>)
+    requires xs == ys
+    ensures to_nat(xs) == to_nat(ys)
+  {
+    reveal to_nat();
   }
 
   /* Proves the nat representation of a sequence is bounded by BASE to the
   power of the sequence length. */
-  lemma lemma_to_nat_bound(xs: seq<BaseType>)
+  lemma lemma_seq_nat_bound(xs: seq<BaseType>)
     ensures to_nat(xs) < power(BASE, |xs|)
   {
     reveal to_nat();
@@ -65,7 +70,7 @@ module IntSeq {
       calc {
         to_nat(xs);
         to_nat(drop_last(xs)) + last(xs) * pow;
-        < { lemma_to_nat_bound(drop_last(xs)); }
+        < { lemma_seq_nat_bound(drop_last(xs)); }
         pow + last(xs) * pow;
         <=
           {
@@ -79,24 +84,39 @@ module IntSeq {
     }
   }
 
+  function method {:opaque} prefix_nat(xs: seq<BaseType>, i: nat): nat
+    requires 0 <= i <= |xs|
+  {
+    to_nat(xs[..i])
+  }
+
+  lemma lemma_prefix_equivalence(xs: seq<BaseType>, ys: seq<BaseType>, i: nat)
+    requires 0 <= i <= |xs| && 0 <= i <= |ys|
+    requires xs[..i] == ys[..i]
+    ensures prefix_nat(xs, i) == prefix_nat(ys, i)
+  {
+    reveal prefix_nat();
+  }
+
   /* Proves the nat representation of a prefix based on a smmaller prefix. */
-  lemma lemma_to_nat_prefix(xs: seq<BaseType>, i: nat)
+  lemma lemma_prefix_nat(xs: seq<BaseType>, i: nat)
     requires 1 <= i < |xs|
-    ensures to_nat(xs[..i]) == to_nat(xs[..i-1]) + xs[i-1] * power(BASE, i - 1)
+    ensures prefix_nat(xs, i)
+         == prefix_nat(xs, i - 1) + xs[i - 1] * power(BASE, i - 1)
   {
     assert xs[..i][..i-1] == xs[..i-1];
+    reveal prefix_nat();
     reveal to_nat();
   }
 
-  // unstable
   /* Proves mod equivalence between the nat representation of a sequence and
   the lsw of the sequence.*/
-  lemma lemma_lsw_mod_equivalence(xs: seq<BaseType>)
+  lemma lemma_seq_lsw_mod_equivalence(xs: seq<BaseType>)
     requires |xs| >= 1;
     ensures is_mod_equivalent(to_nat(xs), xs[0], BASE);
   {
     if |xs| == 1 {
-      lemma_to_nat_len_1(xs);
+      lemma_seq_len_1_nat(xs);
     } else {
       assert is_mod_equivalent(to_nat(xs), xs[0], BASE) by {
         var len' := |xs| - 1;
@@ -113,12 +133,29 @@ module IntSeq {
               assert is_mod_equivalent(last(xs) * pow, 0, BASE);
             }
           is_mod_equivalent(to_nat(xs), to_nat(xs'), BASE);
-            { lemma_lsw_mod_equivalence(xs'); }
+            { lemma_seq_lsw_mod_equivalence(xs'); }
           is_mod_equivalent(to_nat(xs), xs[0], BASE);
         }
       }
     }
   }
+
+  //////////////////////////////////////////////////////////////////////////////
+  //
+  // to_seq definition and lemmas
+  //
+  //////////////////////////////////////////////////////////////////////////////
+
+  /* Converts a nat to a sequence. */
+  function method {:opaque} to_seq(x: nat): seq<BaseType>
+    decreases x
+  {
+    if x == 0 then []
+    else
+      lemma_div_basics_auto();
+      to_seq(x / BASE) + [x % BASE]
+  }
+
 
   //////////////////////////////////////////////////////////////////////////////
   //
@@ -134,7 +171,7 @@ module IntSeq {
   }
 
   /* nat representation of an all zero sequence is 0. */
-  lemma lemma_seq_zero_to_nat(len: nat)
+  lemma lemma_seq_zero_nat(len: nat)
     ensures to_nat(seq_zero(len)) == 0
   {
     reveal to_nat();
@@ -145,7 +182,7 @@ module IntSeq {
         to_nat(seq_zero(len - 1) + [0]);
         to_nat(seq_zero(len - 1)) + 0 * power(BASE, len - 1);
           {
-            lemma_seq_zero_to_nat(len - 1);
+            lemma_seq_zero_nat(len - 1);
             lemma_mul_basics_auto();
           }
         0;
@@ -155,7 +192,7 @@ module IntSeq {
 
   /* Adding a zero as the least significant bit is equal to multiplying the
   number by BASE. */
-  lemma lemma_to_nat_zero_prepend(xs: seq<BaseType>)
+  lemma lemma_seq_prepend_zero(xs: seq<BaseType>)
     ensures to_nat([0] + xs) == to_nat(xs) * BASE
   {
     reveal to_nat();
@@ -166,7 +203,7 @@ module IntSeq {
         to_nat([0] + xs);
           { assert drop_last([0] + xs) == [0] + drop_last(xs); }
         to_nat([0] + drop_last(xs)) + last(xs) * power(BASE, |xs|);
-          { lemma_to_nat_zero_prepend(drop_last(xs)); }
+          { lemma_seq_prepend_zero(drop_last(xs)); }
         to_nat(drop_last(xs)) * BASE + last(xs) * power(BASE, |xs|);
           {
             reveal power();
@@ -180,7 +217,7 @@ module IntSeq {
 
   /* Adding zero(s) as the most significant bit(s) does not change the value of
   the number. */
-  lemma lemma_to_nat_zero_extend(xs': seq<BaseType>, xs: seq<BaseType>) 
+  lemma lemma_seq_append_zero(xs': seq<BaseType>, xs: seq<BaseType>) 
     requires |xs'| < |xs|
     requires var len' := |xs'|;
       && drop_last(xs) == xs'
@@ -194,7 +231,7 @@ module IntSeq {
         to_nat(xs);
         to_nat(drop_last(xs)) + last(xs) * power(BASE, len - 1);
         to_nat(drop_last(xs));
-          { lemma_to_nat_zero_extend(xs', drop_last(xs)); }
+          { lemma_seq_append_zero(xs', drop_last(xs)); }
         to_nat(xs');
       }
     }
@@ -207,38 +244,38 @@ module IntSeq {
   //////////////////////////////////////////////////////////////////////////////
 
   /* Adds two sequences. */
-  function method {:opaque} seq_addc(xs: seq<BaseType>,
-                                     ys: seq<BaseType>): (seq<BaseType>, nat)
+  function method {:opaque} seq_add(xs: seq<BaseType>,
+                                    ys: seq<BaseType>): (seq<BaseType>, nat)
     requires |xs| == |ys|
-    ensures var (zs, cout) := seq_addc(xs, ys); |zs| == |xs|
+    ensures var (zs, cout) := seq_add(xs, ys); |zs| == |xs|
   {
-    reveal seq_addc();
+    reveal seq_add();
     if |xs| == 0 then ([], 0)
     else
-      var (zs', cin) := seq_addc(drop_last(xs), drop_last(ys));
+      var (zs', cin) := seq_add(drop_last(xs), drop_last(ys));
       var sum: int := last(xs) + last(ys) + cin;
       var (sum_out, cout) := if sum < BASE then (sum, 0) else (sum - BASE, 1);
       (zs' + [sum_out], cout)
   }
 
-  /* Proves seq_addc yields the same value as converting the sequences to nats,
+  /* Proves seq_add yields the same value as converting the sequences to nats,
   then adding them. */
-  lemma lemma_seq_addc_nat(xs: seq<BaseType>,
-                           ys: seq<BaseType>,
-                           zs: seq<BaseType>,
-                           cout: nat)
+  lemma lemma_seq_add_nat(xs: seq<BaseType>,
+                          ys: seq<BaseType>,
+                          zs: seq<BaseType>,
+                          cout: nat)
     requires |xs| == |ys|
-    requires seq_addc(xs, ys) == (zs, cout)
+    requires seq_add(xs, ys) == (zs, cout)
     ensures to_nat(xs) + to_nat(ys) == to_nat(zs) + cout * power(BASE, |xs|)
   {
-    reveal seq_addc();
+    reveal seq_add();
     reveal to_nat();
     if |xs| == 0 {
       reveal power();
     } else {
       var len' := |xs| - 1;
       var pow := power(BASE, len');
-      var (zs', cin) := seq_addc(drop_last(xs), drop_last(ys));
+      var (zs', cin) := seq_add(drop_last(xs), drop_last(ys));
       var sum: int := last(xs) + last(ys) + cin;
       var z := if sum < BASE then sum else sum - BASE;
       assert sum == z + cout * BASE;
@@ -246,7 +283,7 @@ module IntSeq {
       calc {
         to_nat(zs);
         to_nat(zs') + z * pow;
-          { lemma_seq_addc_nat(drop_last(xs), drop_last(ys), zs', cin); }
+          { lemma_seq_add_nat(drop_last(xs), drop_last(ys), zs', cin); }
         to_nat(drop_last(xs)) + to_nat(drop_last(ys)) - cin * pow + z * pow;
           {
             lemma_mul_equality_auto();
@@ -264,60 +301,60 @@ module IntSeq {
   }
 
   /* Subtracts two sequences. */
-  function method {:opaque} seq_subb(xs: seq<BaseType>,
-                                     ys: seq<BaseType>): (seq<BaseType>, nat)
+  function method {:opaque} seq_sub(xs: seq<BaseType>,
+                                    ys: seq<BaseType>): (seq<BaseType>, nat)
     requires |xs| == |ys|
-    ensures var (zs, bout) := seq_subb(xs, ys); |zs| == |xs|
+    ensures var (zs, cout) := seq_sub(xs, ys); |zs| == |xs|
   {
-    reveal seq_subb();
+    reveal seq_sub();
     if |xs| == 0 then ([], 0)
     else 
-      var (zs, bin) := seq_subb(drop_last(xs), drop_last(ys));
-      var (diff_out, bout) := if last(xs) >= last(ys) + bin
-                              then (last(xs) - last(ys) - bin, 0)
-                              else (BASE + last(xs) - last(ys) - bin, 1);
-      (zs + [diff_out], bout)
+      var (zs, cin) := seq_sub(drop_last(xs), drop_last(ys));
+      var (diff_out, cout) := if last(xs) >= last(ys) + cin
+                              then (last(xs) - last(ys) - cin, 0)
+                              else (BASE + last(xs) - last(ys) - cin, 1);
+      (zs + [diff_out], cout)
   }
 
-  /* Proves seq_subb yields the same value as converting the sequences to nats,
+  /* Proves seq_sub yields the same value as converting the sequences to nats,
   then subtracting them. */
-  lemma lemma_seq_subb_nat(xs: seq<BaseType>,
-                           ys: seq<BaseType>,
-                           zs: seq<BaseType>,
-                           bout: nat)
+  lemma lemma_seq_sub_nat(xs: seq<BaseType>,
+                          ys: seq<BaseType>,
+                          zs: seq<BaseType>,
+                          cout: nat)
     requires |xs| == |ys|
-    requires seq_subb(xs, ys) == (zs, bout)
-    ensures to_nat(xs) - to_nat(ys) + bout * power(BASE, |xs|) == to_nat(zs)
+    requires seq_sub(xs, ys) == (zs, cout)
+    ensures to_nat(xs) - to_nat(ys) + cout * power(BASE, |xs|) == to_nat(zs)
   {
-    reveal seq_subb();
+    reveal seq_sub();
     reveal to_nat();
     if |xs| == 0 {
       reveal power();
     } else {
       var len' := |xs| - 1;
       var pow := power(BASE, len');
-      var (zs', bin) := seq_subb(drop_last(xs), drop_last(ys));
-      var z := if last(xs) >= last(ys) + bin
-               then last(xs) - last(ys) - bin
-               else BASE + last(xs) - last(ys) - bin;
-      assert bout * BASE + last(xs) - bin - last(ys) == z;
+      var (zs', cin) := seq_sub(drop_last(xs), drop_last(ys));
+      var z := if last(xs) >= last(ys) + cin
+               then last(xs) - last(ys) - cin
+               else BASE + last(xs) - last(ys) - cin;
+      assert cout * BASE + last(xs) - cin - last(ys) == z;
       
       calc {
         to_nat(zs);
         to_nat(zs') + z * pow;
-          { lemma_seq_subb_nat(drop_last(xs), drop_last(ys), zs', bin); }
-        to_nat(drop_last(xs)) - to_nat(drop_last(ys)) + bin * pow + z * pow;
+          { lemma_seq_sub_nat(drop_last(xs), drop_last(ys), zs', cin); }
+        to_nat(drop_last(xs)) - to_nat(drop_last(ys)) + cin * pow + z * pow;
           {
             lemma_mul_equality_auto();
-            assert pow * (bout * BASE + last(xs) - bin - last(ys)) == pow * z;
+            assert pow * (cout * BASE + last(xs) - cin - last(ys)) == pow * z;
             lemma_mul_is_distributive_auto();
           }
-        to_nat(xs) - to_nat(ys) + bout * BASE * pow;
+        to_nat(xs) - to_nat(ys) + cout * BASE * pow;
           {
-            lemma_mul_is_associative(bout, BASE, pow);
+            lemma_mul_is_associative(cout, BASE, pow);
             reveal power();
           }
-        to_nat(xs) - to_nat(ys) + bout * power(BASE, |xs|);
+        to_nat(xs) - to_nat(ys) + cout * power(BASE, |xs|);
       }
     }
   }
